project/util/NatMap.v
@@ -1,41 +1,16 @@
 Require Import FMaps.
+Require Export FMapAVL.
 
+(* Instantiate an FMap module, such that it is the same across the whole project *)
 
 Definition Node := Nat_as_OT.t.
 
-Module NatMap := FMapList.Make(Nat_as_OT).
+Print Module FMaps.
 
-Module WF := WFacts_fun Nat_as_OT NatMap. (* Library of useful lemmas about maps *)
-Module WP := WProperties_fun Nat_as_OT NatMap. (* More useful stuff about maps *)
-Print Module WF.
-Print Module WP.
-Check Nat_as_OT.lt. (*   : positive -> positive -> Prop *)
+(* Uses the quick AVL-tree variant *)
+Module NatMap := FMapAVL.Make(Nat_as_OT).
 
-
-
-
-
-Module PairNat_as_OT := PairOrderedType(Nat_as_OT)(Nat_as_OT).
-Definition NodePair := PairNat_as_OT.t.
-
-Module PairNatMap := FMapList.Make(PairNat_as_OT).
-
-Module PWF := WFacts_fun PairNat_as_OT PairNatMap. (* Library of useful lemmas about maps *)
-Module PWP := WProperties_fun PairNat_as_OT PairNatMap. (* More useful stuff about maps *)
-
-
-
-Definition filter_map {A : Type} (pred : PairNatMap.key -> A -> bool) (m : PairNatMap.t A) : PairNatMap.t A :=
-  PairNatMap.fold (fun k v acc =>
-            if pred k v then PairNatMap.add k v acc else acc)
-         m
-         (PairNatMap.empty A)
-.
-
-
-(* Definition myPairNatMap : PairNatMap.t nat := PairNatMap.empty nat.
-Definition myPairNatMap' := PairNatMap.add (1, 2) 3 myPairNatMap.
-Compute PairNatMap.find (1, 2) myPairNatMap'.
-Definition isIn (keys : nat * nat) (map : PairNatMap.t nat) := PairNatMap.In keys map.
-Compute PairNatMap.In (1, 2) myPairNatMap'. *)
-
+(* Library of useful lemmas about maps *)
+Module MFacts := WFacts_fun Nat_as_OT NatMap.
+(* More useful lemmas about maps *)
+Module MProps := WProperties_fun Nat_as_OT NatMap.
