project/util/util.v
@@ -5,78 +5,46 @@ Require Import List.
 Require Import Coq.Sets.Ensembles.
 Require Import Setoid Morphisms.
 
-
-(* Utility things, that don't really belong anywhere else *)
-
-
-(* Defining my own Ensemble operations, as the library ones are really clunky and untransparent *)
-
-(* This works better in proofs than the library Add for ensembles *)
-Definition cEnsembleAdd {A : Type} (a : A) (en : Ensemble A) : Ensemble A :=
-  fun (x : A) => x = a \/ en x
-.
-
-Definition cEnsembleUnion {A : Type} (en1 en2 : Ensemble A) : Ensemble A :=
-  fun (a : A) => en1 a \/ en2 a
-.
+(* Defines miscellaneous utilities useful across the project  *)
 
 
-Definition cListToEnsemble {A : Type} (az : list A) : Ensemble A :=
-  fold_right cEnsembleAdd (Empty_set A) az
-.
+(* Custom additional functions for Ensembles. Standard library equivalents may exist,
+but they are less transparent and more difficult to work with *)
+Definition Ensemble_add {A : Type} (a : A) (en : Ensemble A) : Ensemble A :=
+    fun (x : A) => x = a \/ en x.
 
-Definition cEnsemble_equiv {A : Type} (en1 en2 : Ensemble A) : Prop :=
-  forall a, en1 a <-> en2 a
-.
-
-Notation "en1 S== en2" := (cEnsemble_equiv en1 en2) (at level 100, right associativity).
-
-Instance Ensemble_Equivalence {A : Type} : Equivalence (@cEnsemble_equiv A).
-Proof.
-  unfold cEnsemble_equiv. firstorder.
-Qed.
+Definition Ensemble_union {A : Type} (en1 en2 : Ensemble A) : Ensemble A :=
+    fun (a : A) => en1 a \/ en2 a.
 
 
 
-(* Lemma fold_right_preserves_invariant:
-  forall (A B C : Type) (f : A -> B -> B) (g : B -> C),
-    (forall a b, g (f a b) = g b) ->
-    forall l b0, g (fold_right f b0 l) = g b0.
-Proof.
-  intros. induction l; simpl.
-  - reflexivity.
-  - rewrite H. apply IHl.
-Qed.
- *)
-
-
-
-
-(* This is from software foundations. Eventually, I will move this somewhere else *)
+(* Leads to define "bdestruct", a useful tactic from
+Software Foundations, Volume 3: Verified Functional Algorithms, Chapter Perm *)
 Lemma eqb_reflect : forall x y, reflect (x = y) (x =? y).
 Proof.
-  intros x y. apply iff_reflect. symmetry.
-  apply Nat.eqb_eq.
+    intros x y. apply iff_reflect. symmetry.
+    apply Nat.eqb_eq.
 Qed.
+
 Lemma ltb_reflect : forall x y, reflect (x < y) (x <? y).
 Proof.
-  intros x y. apply iff_reflect. symmetry.
-  apply Nat.ltb_lt.
+    intros x y. apply iff_reflect. symmetry.
+    apply Nat.ltb_lt.
 Qed.
+
 Lemma leb_reflect : forall x y, reflect (x <= y) (x <=? y).
 Proof.
-  intros x y. apply iff_reflect. symmetry.
-  apply Nat.leb_le.
+    intros x y. apply iff_reflect. symmetry.
+    apply Nat.leb_le.
 Qed.
 
 Hint Resolve ltb_reflect leb_reflect eqb_reflect : bdestruct.
+
 Ltac bdestruct X :=
-  let H := fresh in let e := fresh "e" in
-   evar (e: Prop);
-   assert (H: reflect e X); subst e;
-    [ auto with bdestruct
-    | destruct H as [H|H];
-       [ | try first [apply not_lt in H | apply not_le in H]]].
-
-
-       
+    let H := fresh in let e := fresh "e" in
+        evar (e: Prop);
+        assert (H: reflect e X); subst e;
+        [ auto with bdestruct
+        | destruct H as [H|H];
+            [ | try first [apply not_lt in H | apply not_le in H]]
+        ].
