project/relational_graph.v
@@ -5,25 +5,25 @@ Require Import Coq.Sets.Ensembles.
 Require Import MyProject.project.util.NatSet.
 Require Import MyProject.project.util.util.
 
-
 Require Import List.
 Import ListNotations.
 
 
+(* Defining a relational_graph (RG) and its operations. It it most similar to the typical graph from discrete mathematics.
+It is useful as a model for verification. *)
 
-
-(* Defining a Relational Graph and its (possible) operations *)
 
 Definition _edgeRelation (A B : Type) := A -> A -> B -> Prop.
 
 Definition _unlabelEdgeRelation {A B: Type} (edges : _edgeRelation A B) : relation A :=
-    fun (a1 a2 : A) => exists (l: B), edges a1 a2 l.
+    fun (a1 a2 : A) => exists (l : B), edges a1 a2 l.
 
+
+(* Edges can only connect _existing_ nodes *)
 Definition _valid_cond {A B : Type} (nodes : Ensemble A) (edges : _edgeRelation A B) : Prop :=
     forall (a1 a2 : A) (b : B), edges a1 a2 b -> nodes a1 /\ nodes a2.
 
 
-(* Is is possible to write operations "on" it, but as soon as you want to write a function that would return some "result", things get complicated *)
 Record RG (A B : Type) := {
     RG_nodes : Ensemble A;
     RG_edges : _edgeRelation A B;
@@ -34,30 +34,25 @@ Arguments RG_nodes {A B}.
 Arguments RG_edges {A B}.
 Arguments RG_valid {A B}.
 
-
+(* Trivialize proving of _valid_cond in most cases *)
 Ltac RG_valid_prover := unfold _valid_cond; firstorder.
 Ltac RG_valid_prover_with rg := pose proof rg.(RG_valid); RG_valid_prover.
 Ltac RG_valid_prover_withs rg1 rg2 := pose proof rg1.(RG_valid); RG_valid_prover_with rg2.
 
-(* Two relational graphs are "the same", when their Ensemble and relation are the same *)
+
+(* Two relational graphs are "the same", when their Ensemble and relation are the same. *)
 Definition RG_equiv {A B : Type} (rg1 rg2 : RG A B) : Prop :=
     (* The first condition is definitely needed, as we can have "singleton" graphs *)
     (forall (a : A), rg1.(RG_nodes) a <-> rg2.(RG_nodes) a)
-    /\ (forall (a1 a2 : A) (b : B), rg1.(RG_edges) a1 a2 b <-> rg2.(RG_edges) a1 a2 b)
-.
+        /\ (forall (a1 a2 : A) (b : B), rg1.(RG_edges) a1 a2 b <-> rg2.(RG_edges) a1 a2 b).
+
 Notation "g1 === g2" := (RG_equiv g1 g2) (at level 100, right associativity).
 
-
+(* A variant with only single edges *)
 Definition RG_unlE (A : Type) := RG A unit.
-(* The followign two don't actually make sense, since one needs a node type for... well nodes to exists *)
-(* Definition RG_unlN (B : Type) := RG unit B.
-Definition RG_unl (B : Type) := RG unit unit. *)
 
 
-
-
-(* Defining fundamental Operations on RGs: *)
-
+(* Start defining operations: *)
 Definition RG_empty {A B : Type} : RG A B.
 Proof.
     refine {|
@@ -69,8 +64,7 @@ Proof.
 Defined.
 
 Definition RG_isEmpty {A B: Type} (rg : RG A B) : Prop :=
-    forall (a : A), rg.(RG_nodes) a <-> False
-.
+    forall (a : A), rg.(RG_nodes) a <-> False.
 
 
 Definition RG_addNode {A B : Type} (node : A) (rg : RG A B) : RG A B.
@@ -88,8 +82,8 @@ Definition RG_addEdge {A B : Type} (from to : A) (label : B) (rg : RG A B) : RG 
 Proof.
     refine {|
         RG_nodes := fun a => (RG_addNode to (RG_addNode from rg)).(RG_nodes) a;
-        RG_edges := fun a1 a2 l =>  (a1 = from /\ a2 = to /\ l = label) \/
-                                    rg.(RG_edges) a1 a2 l;
+        RG_edges := fun a1 a2 l => (a1 = from /\ a2 = to /\ l = label)
+                                        \/ rg.(RG_edges) a1 a2 l;
         RG_valid := _
     |}.    
     RG_valid_prover_with rg.
@@ -113,8 +107,8 @@ Definition RG_removeEdge {A B : Type} (from to : A) (label : B) (rg : RG A B) : 
 Proof.
     refine {|
         RG_nodes := rg.(RG_nodes);
-        RG_edges := fun a1 a2 l =>  not (a1 = from /\ a2 = to /\ l = label) /\
-                                    rg.(RG_edges) a1 a2 l;
+        RG_edges := fun a1 a2 l => not (a1 = from /\ a2 = to /\ l = label)
+                                    /\ rg.(RG_edges) a1 a2 l;
         RG_valid := _
     |}.
     RG_valid_prover_with rg.
@@ -129,10 +123,8 @@ Definition RG_getIncomingEdges {A B : Type} (node : A) (rg : RG A B) : _edgeRela
     fun (a1 a2 : A) l => rg.(RG_edges) a1 a2 l /\ a2 = node.
 
 Definition RG_getIncidentEdges {A B : Type} (node : A) (rg : RG A B) : _edgeRelation A B :=
-    fun (a1 a2 : A) l =>    (RG_getOutgoingEdges node rg) a1 a2 l \/
-                            (RG_getIncomingEdges node rg) a1 a2 l.
-
-(* There can also be variations of this, where you the the neighbor nodes and not just edges ... *)
+    fun (a1 a2 : A) l => (RG_getOutgoingEdges node rg) a1 a2 l
+                            \/ (RG_getIncomingEdges node rg) a1 a2 l.
 
 
 
@@ -147,33 +139,9 @@ Proof.
 Defined.
 
 
-(* Connectedness *)
 Definition RG_existsPath {A B : Type} (node1 node2 : A) (rg : RG A B) : Prop :=
     clos_trans A (_unlabelEdgeRelation rg.(RG_edges)) node1 node2.
 
-
+(* Is node reachable from froms in exactly a single step? *)
 Definition RG_reachableInOneStep {A B : Type} (froms : Ensemble A) (node : A) (rg : RG A B) : Prop :=
     exists from l, froms from /\ rg.(RG_edges) from node l.
-
-(* Start implementing search *)
-
-
-(* From CertiGraph *)
-(* Context {Vertex Edge: Type}.
-
-Record PreGraph {EV: EqDec Vertex eq} {EE: EqDec Edge eq} := {
-  vvalid : Ensemble Vertex;
-  evalid : Ensemble Edge;
-  src : Edge -> Vertex;
-  dst : Edge -> Vertex
-}.
-
-Context {EV: EqDec Vertex eq}.
-Context {EE: EqDec Edge eq}.
-
-Record LabeledGraph {DV DE DG: Type} := {
-  pg_lg: PreGraph;
-  vlabel: Vertex -> DV;
-  elabel: Edge -> DE;
-  glabel: DG
-}. *)
