project/relational_graph_theory.v
@@ -1,70 +1,49 @@
-Require Import Coq.Relations.Relation_Definitions.
-Require Import Coq.Relations.Relation_Operators.
-Require Import Coq.Sets.Ensembles.
+Require Import Setoid Morphisms.
 
 Require Import MyProject.project.relational_graph.
 
-(* Stated and proves Lemmas and Theorems about RGs *)
+(* Stating and proving Lemmas and Theorems about RGs *)
+
 
 (* "RG_equiv" is an equivalence relation: *)
-(* Reflexive *)
-Theorem RG_equiv_Reflexive {A B : Type}: forall (rg : RG A B), RG_equiv rg rg.
-Proof.
-    firstorder.
-Qed.
-    
-
-(* Symmetric *)
-Theorem RG_equiv_Symmetric {A B : Type}: forall (rg1 rg2 : RG A B), RG_equiv rg1 rg2 <-> RG_equiv rg2 rg1.
-Proof.
-    firstorder.
-Qed. 
-
-(* Transitive *)
-Theorem RG_equiv_Transitive {A B : Type}: forall (rg1 rg2 rg3 : RG A B), RG_equiv rg1 rg2 -> RG_equiv rg2 rg3 -> RG_equiv rg1 rg3.
-Proof.
-    firstorder.
-    - apply H1. apply H2. apply H3.
-    - apply H2. apply H1. apply H3.
-Qed.
-
-(* Section to make rewrite work with equiv_RG *)
-
-(* Source for rewrite: https://stackoverflow.com/questions/56099646/use-rewrite-tactic-with-my-own-operator-in-coq *)
-Require Import Setoid Morphisms.
 Instance RG_Equivalence {A B : Type} : Equivalence (@RG_equiv A B).
 Proof.
     unfold RG_equiv. split.
-    - unfold Reflexive. intros. pose proof (@RG_equiv_Reflexive A). apply H.
-    - unfold Symmetric. intros. pose proof (@RG_equiv_Symmetric A). apply H0. apply H.
-    - unfold Transitive. intros. pose proof (@RG_equiv_Transitive A B). apply (H1 x y).
-        + apply H.
-        + apply H0.
+    (* Reflexive *)
+    - firstorder.
+    (* Symmetric *)
+    - firstorder.
+    (* Transitive *)
+    - unfold Transitive. firstorder.
+        + apply H1. apply H2. assumption.
+        + apply H2. apply H1. assumption.
 Qed.
 
-(* Does something very similar as the proof above, but uses "other evidence" for equivalence *)
+
+
+(* Proves a relation derived from RG_equiv (off by just a coercion) is also an equivalence relation *)
 Ltac G_derived_equivalence_prover A B f :=
-  pose proof (@RG_Equivalence A B) as H;
-  destruct H as [Eq_Refl Eq_Symm Eq_Trans]; split;
-  [ unfold Reflexive; intros; unfold Reflexive in Eq_Refl; apply Eq_Refl
-  | unfold Symmetric; intros; unfold Symmetric in Eq_Symm; apply Eq_Symm; apply H
-  | unfold Transitive; intros x y z H H0; intros; unfold Transitive in Eq_Trans; apply (Eq_Trans _ (f y) _);
-    [ apply H
-    | apply H0
-    ]
-  ].
+    pose proof (@RG_Equivalence A B) as H;
+    destruct H as [Eq_Refl Eq_Symm Eq_Trans]; split;
+    [ unfold Reflexive; intros; unfold Reflexive in Eq_Refl; apply Eq_Refl
+    | unfold Symmetric; intros; unfold Symmetric in Eq_Symm; apply Eq_Symm; apply H
+    | unfold Transitive; intros x y z H H0; intros; unfold Transitive in Eq_Trans; apply (Eq_Trans _ (f y) _);
+        [ apply H
+        | apply H0
+        ]
+    ].
 
 
-(* This demonstrated the utility of the model :) *)
+(* Some theorems about RG_transpose: *)
 Theorem RG_transpose_transpose {A B : Type}: forall (rg : RG A B), RG_transpose (RG_transpose rg) === rg.
 Proof.
-  firstorder.
+    firstorder.   
 Qed.
 
 Theorem RG_transpose_same_nodes {A B : Type}: forall (rg : RG A B) n,
   (RG_transpose rg).(RG_nodes) n <-> rg.(RG_nodes) n.
 Proof.
-  firstorder.
+    firstorder.
 Qed.
 
 Theorem RG_transpose_flips_edges {A B : Type}: forall (rg : RG A B) n1 n2 l,
@@ -79,4 +58,3 @@ Proof.
   intros.
   apply Operators_Properties.clos_trans_transp_permute.
 Qed.
-
