project/util/NatSet.v
@@ -1,10 +1,14 @@
-Require Import FSets.
+Require Import MSets.
 
-(* TODO: migrate to Msets *)
+(* Instantiate an FSet module, such that it is the same across the whole project *)
+
+
 Definition Node := Nat_as_OT.t.
 
-Module NatSet := FSetList.Make(Nat_as_OT).
-Module NatSetProperties := EqProperties(NatSet).
+(* Uses the quick AVL-tree variant *)
+Module NatSet := MSetAVL.Make(Nat_as_OT).
+Module SProps := EqProperties(NatSet).
 
+(* Custom additional function for NatSets "fromList" *)
 Definition NatSet_fromList (l : list Node) : NatSet.t :=
     fold_right NatSet.add NatSet.empty l.
